Fix extraction with Guido's help

io/case-study/Monitor.fst
@@ -6,12 +6,12 @@ open Utils
 
 private
 val monitor_state : ref mymst.cst
-let monitor_state = ST.alloc mymst.init_cst
+let monitor_state = ST.alloc my_init_cst
 
 let get_state () : St mymst.cst = !monitor_state
 
 let update_state caller (cmd:io_cmds) (argz:io_sig.args cmd) (rez:io_sig.res cmd argz) : St unit =
   let s0 = get_state () in
   let e = convert_call_to_event caller cmd argz rez in
-  let s1 = mymst.update_cst s0 e in
+  let s1 = my_update_cst s0 e in
   monitor_state := s1
